ulib/FStar.Tactics.fst
@@ -9,32 +9,30 @@ type typ     = term
 type binders = list binder
 type goal    = env * term
 type goals   = list goal
-type state   = goals  //active goals 
+type state   = goals  //active goals
              * goals  //goals that have to be dispatched to SMT: maybe change this part of the state to be opaque to a user program
 
 (* This is meant to be all named representation
-     -- while providing some conveniences for 
-        handling the logical structure of a term 
+     -- while providing some conveniences for
+        handling the logical structure of a term
    NB: rename this to term_view? or something like that
 *)
 
-#reset-options "--no_tactics"
-
-noeq type formula = 
+noeq type formula =
   //the logical skeleton of a term
   | True_  : formula
-  | False_ : formula  
+  | False_ : formula
   | Eq     : typ -> term -> term -> formula
   | And    : term -> term -> formula  //Prims.l_and
   | Or     : term -> term -> formula
   | Not    : term -> formula
   | Implies: term -> term -> formula
-  | Iff    : term -> term -> formula  
+  | Iff    : term -> term -> formula
   | Forall : binders -> term -> formula
   | Exists : binders -> term -> formula
   | App    : term -> term -> formula
   | Name   : binder -> formula
-   (* TODO more cases *) 
+   (* TODO more cases *)
   | IntLit : int -> formula
   //Abs   : binders -> term -> formula //Named repr
   //Match : ....
@@ -62,8 +60,6 @@ noeq type __result (a:Type) =
   | Success: a -> state -> __result a
   | Failed: string -> state -> __result a
 
-(* If it starts with an underline don't use it from the outside! *)
-
 let __tac (a:Type) = state -> M (__result a)
 
 (* monadic return *)
@@ -78,9 +74,9 @@ let __bind (a:Type) (b:Type) (t1:__tac a) (t2:a -> __tac b) : __tac b =
              | Failed msg q -> Failed msg q
 
 (* Actions *)
-let __get () : __tac state = fun s0 -> Success s0 s0 
+let __get () : __tac state = fun s0 -> Success s0 s0
 
-let tac_wp a = state -> (__result a -> Tot Type0) -> Tot Type0
+let __tac_wp a = state -> (__result a -> Tot Type0) -> Tot Type0
 
 (*
  * The DMFF-generated `bind_wp` doesn't the contain the "don't duplicate the post-condition"
@@ -88,15 +84,15 @@ let tac_wp a = state -> (__result a -> Tot Type0) -> Tot Type0
  *
  * Work around that by overriding `bind_wp` for the effect with an efficient one.
  *)
-unfold let g_bind (a:Type) (b:Type) (wp:tac_wp a) (f:a -> tac_wp b) = fun ps post ->
+unfold let g_bind (a:Type) (b:Type) (wp:__tac_wp a) (f:a -> __tac_wp b) = fun ps post ->
     wp ps (fun m' -> match m' with
                      | Success a q -> f a q post
                      | Failed msg q -> post (Failed msg q))
 
-unfold let g_compact (a:Type) (wp:tac_wp a) : tac_wp a =
+unfold let g_compact (a:Type) (wp:__tac_wp a) : __tac_wp a =
     fun ps post -> wp ps (fun _ -> True) /\ (forall (r:__result a). post r \/ wp ps (fun r' -> ~(r == r')))
 
-unfold let __TAC_eff_override_bind_wp (r:range) (a:Type) (b:Type) (wp:tac_wp a) (f:a -> tac_wp b) =
+unfold let __TAC_eff_override_bind_wp (r:range) (a:Type) (b:Type) (wp:__tac_wp a) (f:a -> __tac_wp b) =
     g_compact b (g_bind a b wp f)
 
 (* total  *) //disable the termination check, although it remains reifiable
@@ -110,6 +106,12 @@ reifiable reflectable new_effect {
 effect Tac (a:Type) = TAC a (fun i post -> forall j. post j)
 let tactic (a:Type) = unit -> Tac a
 
+let return (#a:Type) (x:a) : tactic a =
+    fun () -> x
+
+let bind (#a:Type) (#b:Type) (t : tactic a) (f : a -> tactic b) : tactic b =
+    fun () -> let r = t () in f r ()
+
 (* working around #885 *)
 let __fail (a:Type) (msg:string) : __tac a = fun s0 -> Failed #a msg s0
 let fail (#a:Type) (msg:string) : tactic a = fun () -> TAC?.reflect (__fail a msg)
@@ -117,35 +119,22 @@ let fail (#a:Type) (msg:string) : tactic a = fun () -> TAC?.reflect (__fail a ms
 let reify_tactic (t:tactic 'a) : __tac 'a =
   fun s -> reify (t ()) s
 
-// TODO: SERIOUS: if I use `reify (t1 ()) p` down here, the combination
-// never backtracks. Must be related to the normalization of `reify`, but it's
-// weird anyway that going via reify_tactic "fixes" it
-let or_else (#a:Type) (t1:tactic a) (t2:tactic a) : tactic a = fun () ->
-    TAC?.reflect (fun p -> match reify_tactic t1 p with
-                           | Failed _ _ -> reify_tactic t2 p
-                           | q -> q)
+// Never fails
+let trytac (#a:Type) (t : tactic a) : tactic (option a) = fun () ->
+    TAC?.reflect (fun ps -> match reify_tactic t ps with
+                            | Success a ps' -> Success (Some a) ps'
+                            | Failed _ _ -> Success None ps)
 
-// TODO: forgot the underscore in result and F* blew up,
-// didn't mention a undefined "result". bug?
-abstract 
-let by_tactic (t:state -> __result unit) (a:Type) : Type = a
-
-// Must run with tactics off, as it will otherwise try to run `by_tactic
-// (reify_tactic t)`, which fails as `t` is not a concrete tactic
-#reset-options "--no_tactics"
-let assert_by_tactic (t:tactic unit) (p:Type)
-  : Pure unit 
-         (requires (by_tactic (reify_tactic t) p))
-         (ensures (fun _ -> p))
-  = ()
-#reset-options ""
-
-// TODO: naming convention.. underscore before or after?
+let or_else (#a:Type) (t1 : tactic a) (t2 : tactic a) : tactic a =
+    r <-- trytac t1;
+    (match r with
+    | Some x -> return x
+    | None -> t2)
 
 assume private val __binders_of_env : env -> binders
 let binders_of_env (e:env) : tactic binders = fun () -> __binders_of_env e
 
-assume private val __type_of_binder: binder -> term 
+assume private val __type_of_binder: binder -> term
 let type_of_binder (b:binder) : tactic term = fun () -> __type_of_binder b
 
 assume private val __term_eq : term -> term -> bool
@@ -164,11 +153,11 @@ let inspect t : tactic term_view = fun () -> match __inspect t with
                                              | Some x -> x
                                              | None -> fail "inspect failed, possibly unknown syntax" ()
 
-(* Many of these could be derived from apply_lemma, 
-   rather than being assumed as primitives. 
-   E.g., forall_intros could be an application of 
+(* Many of these could be derived from apply_lemma,
+   rather than being assumed as primitives.
+   E.g., forall_intros could be an application of
          FStar.Classical.forall_intro
- *)         
+ *)
 assume private val __forall_intros: __tac binders
 let forall_intros : tactic binders = fun () -> TAC?.reflect __forall_intros
 
@@ -190,7 +179,8 @@ let split : tactic unit = fun () -> TAC?.reflect __split
 assume private val __merge   : __tac unit
 let merge : tactic unit = fun () -> TAC?.reflect __merge
 
-// TODO: isn't this is unsound if b is not the environment? I think so but couldn't quickly come up with a contradiction
+// TODO: isn't this is unsound if b is not the environment?
+// I think so but couldn't quickly come up with a contradiction
 assume private val __rewrite : binder -> __tac unit
 let rewrite (b:binder) : tactic unit = fun () -> TAC?.reflect (__rewrite b)
 
@@ -205,7 +195,7 @@ let focus (f:tactic unit) : tactic unit = fun () -> TAC?.reflect (__focus (reify
 
 (* could be implemented using __focus *)
 assume private val __seq : __tac unit -> __tac unit -> __tac unit
-let seq (f:tactic unit) (g:tactic unit) : tactic unit = fun () -> 
+let seq (f:tactic unit) (g:tactic unit) : tactic unit = fun () ->
   TAC?.reflect (__seq (reify_tactic f) (reify_tactic g))
 
 assume private val __exact : term -> __tac unit
@@ -218,150 +208,149 @@ assume val __print : string -> __tac unit
 let print (msg:string) : tactic unit = fun () -> TAC?.reflect (__print msg)
 
 assume val __grewrite : term -> term -> __tac unit
-let grewrite (e1:tactic term) (e2:tactic term) : tactic unit =
-    fun () -> let t1 = e1 () in
-              let t2 = e2 () in
-              TAC?.reflect (__grewrite t1 t2)
+let grewrite (t1:term) (t2:term) : tactic unit =
+    fun () -> TAC?.reflect (__grewrite t1 t2)
 
-let tret (#a:Type) (x:a) : tactic a =
-    fun () -> x
+let rec revert_all (bs:binders) : tactic unit =
+    match bs with
+    | [] -> return ()
+    | _::tl -> revert;;
+               revert_all tl
 
-let tbind (#a:Type) (#b:Type) (t : tactic a) (f : a -> tactic b) : tactic b =
-    fun () -> let r = t () in f r ()
-
-let tbind' (#a:Type) (#b:Type) (t : tactic a) (f : tactic b) : tactic b =
-    fun () -> let r = t () in f ()
-
-// For some reason, a direct definition fails.
-let revert_all (bs:binders) : tactic unit =
-    let rec __revert_all (bs:binders) : Tac unit =
-      match bs with
-      | [] -> ()
-      | _::tl -> let _ = revert () in __revert_all tl
-    in fun () -> __revert_all bs
-
+(* Cannot eta reduce this... *)
 let get : tactic state = fun () -> TAC?.__get ()
 
-let cur_goal : tactic goal = fun () ->
-  let goals, _ = get () in
+let cur_goal : tactic goal =
+  ps <-- get;
+  let goals, _ = ps in
   match goals with
-  | [] -> fail "No more goals" ()
-  | hd::_ -> hd
+  | [] -> fail "No more goals"
+  | hd::_ -> return hd
 
-let destruct_equality_implication (t:term) : tactic (option (formula * term)) = fun () ->
-  match term_as_formula t () with
-  | Some (Implies lhs rhs) ->
-    let lhs = term_as_formula lhs () in
-    (match lhs with
-     | Some (Eq _ _ _) -> Some (Some?.v lhs, rhs)
-     | _ -> None)
-  | _ -> None
+let destruct_equality_implication (t:term) : tactic (option (formula * term)) =
+    f <-- term_as_formula t;
+    match f with
+    | Some (Implies lhs rhs) ->
+        begin
+        lhs <-- term_as_formula lhs;
+        match f with
+        | Some (Eq _ _ _) -> return (Some (Some?.v lhs, rhs))
+        | _ -> return None
+        end
+    | _ -> return None
 
 // TODO: aux isn't used. wtf?
-// in this one, if the return type is "tactic unit", it complains
-// about not being able to show a decreasing order. again wtf?
 let rec user_visit (callback:tactic unit) : unit -> Tac unit
-    = fun () ->
-         or_else callback (user_visit callback) ()
+    = or_else callback (user_visit callback)
 
-// TODO: Needs to be unit -> Tac unit since it's a let rec.
-let rec simplify_eq_implication : unit -> Tac unit
-  = fun () ->
-    let context, goal_t = cur_goal () in  // G |- x=e ==> P
-    match destruct_equality_implication goal_t () with
-    | None -> fail "Not an equality implication" ()
+// Need to thunk it like to this for proper handling of non-termination.
+// (not doing it would still work, because of issue #1017, but should not)
+let rec simplify_eq_implication (u:unit) : Tac unit = (
+    g <-- cur_goal;
+    let context, goal_t = g in // G |- x=e ==> P
+    r <-- destruct_equality_implication goal_t;
+    match r with
+    | None ->
+        fail "Not an equality implication"
     | Some (_, rhs) ->
-      let eq_h = implies_intro () in  // G, eq_h:x=e |- P
-      rewrite eq_h (); // G, eq_h:x=e |- P[e/x]
-      clear ();     // G |- P[e/x]
-      user_visit simplify_eq_implication ()
+        eq_h <-- implies_intro; // G, eq_h:x=e |- P
+        rewrite eq_h;; // G, eq_h:x=e |- P[e/x]
+        clear;; // G |- P[e/x]
+        user_visit simplify_eq_implication) ()
 
-let rec try_rewrite_equality (x:term)
-                             (bs:binders)
-  : tactic unit
-  = fun () ->
+let rec try_rewrite_equality (x:term) (bs:binders) : tactic unit =
     match bs with
-    | [] -> ()
-    | x_t::bs -> begin
-      match term_as_formula (type_of_binder x_t ()) () with
-      | Some (Eq _ y _) ->
-        if term_eq x y ()
-        then rewrite x_t ()
-        else try_rewrite_equality x bs ()
-      | _ -> try_rewrite_equality x bs ()
-      end
+    | [] -> return ()
+    | x_t::bs ->
+        t <-- type_of_binder x_t;
+        f <-- term_as_formula t;
+        begin match f with
+        | Some (Eq _ y _) ->
+            b <-- term_eq x y;
+            if b
+            then rewrite x_t
+            else try_rewrite_equality x bs
+        | _ ->
+            try_rewrite_equality x bs
+        end
 
-let rec rewrite_all_context_equalities (bs:binders)
-  : tactic unit
-  = fun () ->
+let rec rewrite_all_context_equalities (bs:binders) : tactic unit =
     match bs with
-    | [] -> ()
+    | [] ->
+        return ()
     | x_t::bs -> begin
-      match term_as_formula (type_of_binder x_t ()) () with
-      | Some (Eq _ _ _) ->
-        rewrite x_t ();
-        rewrite_all_context_equalities bs ()
-      | _ ->
-        rewrite_all_context_equalities bs ()
-      end
+        tx <-- type_of_binder x_t;
+        f <-- term_as_formula tx;
+        match f with
+        | Some (Eq _ _ _) ->
+            rewrite x_t;;
+            rewrite_all_context_equalities bs
+        | _ ->
+            rewrite_all_context_equalities bs
+        end
 
-// TODO: has to be arrow
-let rec rewrite_eqs_from_context : unit -> Tac unit
-  = fun () ->
-       let context, _ = cur_goal () in
-       rewrite_all_context_equalities (binders_of_env context ()) ()
+let rewrite_eqs_from_context : tactic unit =
+    g <-- cur_goal;
+    let context, _ = g in
+    bs <-- binders_of_env context;
+    rewrite_all_context_equalities bs
 
-let rewrite_equality (x:tactic term) : tactic unit
-  = fun () ->
-     let context, _ = cur_goal () in
-     try_rewrite_equality (x ()) (binders_of_env context ()) ()
+let rewrite_equality (x:tactic term) : tactic unit =
+    g <-- cur_goal;
+    let context, _ = g in
+    t <-- x;
+    bs <-- binders_of_env context;
+    try_rewrite_equality t bs
 
-let solved : tactic unit = fun () ->
-  let _, goal = cur_goal () in
-  match term_as_formula goal () with
-  | Some True_ -> ()
-  | _ -> fail "Not solved" ()
+let rewrite_all_equalities : tactic unit =
+    visit (simplify_eq_implication)
 
-let rec just_do_intros : unit -> Tac unit =
-    focus (fun () ->
-       let _ = forall_intros () in
-       let _ = implies_intro () in
-       smt ();
-       revert ();
-       revert ())
-
-// TODO: again has to be an arrow
-let rec rewrite_all_equalities : unit -> Tac unit = fun () ->
-  visit simplify_eq_implication ()
-
-
-assume val lemma_mul_comm : x:nat -> y:nat -> Lemma (op_Multiply x y == op_Multiply y x)
-let mul_commute_ascription : tactic unit
-  = fun () ->
-    let _, goal_t = cur_goal () in  // G |- x=e ==> P
-    match term_as_formula goal_t () with
-    | Some (Eq _ _ _) ->
-      apply_lemma (quote lemma_mul_comm) ()
-    | _ -> fail "Not an equality" ()
-
-// TODO: unfold tactic or complains about termination
-let rec unfold_definition_and_simplify_eq' (tm:term)
-  : unit -> Tac unit
-  = fun () ->
-      let _, goal_t = cur_goal () in  // G |- x=e ==> P
-      match term_as_formula goal_t () with
-      | Some (App hd arg) ->
-        if term_eq hd tm () then trivial ()
-      | _ -> begin
-        match destruct_equality_implication goal_t () with
-        | None -> fail "Not an equality implication" ()
+// See comment on `simplify_eq_implication`
+let rec unfold_definition_and_simplify_eq' (tm:term) (u:unit) : Tac unit = (
+    g <-- cur_goal;
+    let (_, goal_t) = g in
+    f <-- term_as_formula goal_t;
+    match f with
+    | Some (App hd arg) ->
+        b <-- term_eq hd tm;
+        if b
+        then trivial
+        else return ()
+    | _ -> begin
+        r <-- destruct_equality_implication goal_t;
+        match r with
+        | None -> fail "Not an equality implication"
         | Some (_, rhs) ->
-          let eq_h = implies_intro () in  // G, eq_h:x=e |- P
-          rewrite eq_h (); // G, eq_h:x=e |- P[e/x]
-          clear ();     // G |- P[e/x]
-          visit (unfold_definition_and_simplify_eq' tm) ()
-       end
+            eq_h <-- implies_intro;
+            rewrite eq_h;;
+            clear;;
+            visit (unfold_definition_and_simplify_eq' tm)
+        end) ()
 
-let unfold_definition_and_simplify_eq (tm:tactic term) 
-  : tactic unit 
-  = fun () -> unfold_definition_and_simplify_eq' (tm ()) ()
+let unfold_definition_and_simplify_eq (tm:tactic term) : tactic unit =
+    tm' <-- tm;
+    unfold_definition_and_simplify_eq' tm'
+
+abstract
+let by_tactic (t:__tac unit) (a:Type) : Type = a
+
+// Must run with tactics off, as it will otherwise try to run `by_tactic
+// (reify_tactic t)`, which fails as `t` is not a concrete tactic
+#reset-options "--no_tactics"
+let assert_by_tactic (t:tactic unit) (p:Type)
+  : Pure unit
+         (requires (by_tactic (reify_tactic t) p))
+         (ensures (fun _ -> p))
+  = ()
+#reset-options ""
+
+
+(* Monadic helpers, could be made generic for do notation? *)
+
+val liftM2' : ('a -> 'b -> tactic 'c) -> (tactic 'a -> tactic 'b -> tactic 'c)
+let liftM2' f ma mb = a <-- ma;
+                      b <-- mb;
+                      f a b
+
+val liftM2 : ('a -> 'b -> 'c) -> (tactic 'a -> tactic 'b -> tactic 'c)
+let liftM2 f = liftM2' (fun x y -> return (f x y))
